<rdf:RDF xmlns:rdf="http://www.w3.org/1999/02/22-rdf-syntax-ns#"
	xmlns:rdfs="http://www.w3.org/2000/01/rdf-schema#"
	xmlns:owl="http://www.w3.org/2002/07/owl#"
	xmlns:skos="http://www.w3.org/2004/02/skos/core#"
	xmlns="http://gvs.hpl.hp.com/ontologies/services#"
	xml:base="http://gvs.hpl.hp.com/ontologies/services">

	<owl:Class rdf:ID="Service">
		<rdfs:label xml:lang="en">Service</rdfs:label>
		<skos:definition xml:lang="en">
			A service started by the gvs services command
		</skos:definition>
		<rdfs:comment xml:lang="en">the factoryJavaClass property point to an instance of com.hp.hpl.jena.gvs.tool.services.ServiceFactory</rdfs:comment>
		<rdfs:isDefinedBy rdf:resource="" />
	</owl:Class>

	<owl:DatatypeProperty rdf:ID="factoryJavaClass">
		<rdfs:label xml:lang="en">factoryJavaClass</rdfs:label>
		<rdf:type
			rdf:resource="http://www.w3.org/2002/07/owl#FunctionalProperty" />
		<rdfs:range rdf:resource="http://www.w3.org/2001/XMLSchema#string" />
		<rdfs:domain rdf:resource="#Service" />
		<skos:definition xml:lang="en">
			Point to the fully qualified class-name of the service-factory of the subject
		</skos:definition>
	</owl:DatatypeProperty>

	<owl:DatatypeProperty rdf:ID="configuration">
		<rdfs:label xml:lang="en">configuration</rdfs:label>
		<rdf:type
			rdf:resource="http://www.w3.org/2002/07/owl#FunctionalProperty" />
		<rdfs:domain rdf:resource="#Service" />
		<skos:definition xml:lang="en">
			The configuration of the subject
		</skos:definition>
		<rdfs:comment xml:lang="en">Points to a resource of which the description obtained from the trusted sources 
		configures the service. Note that the object must be named so it can be passed to the service.</rdfs:comment>
	</owl:DatatypeProperty>

	<owl:DatatypeProperty rdf:ID="identity">
		<rdfs:label xml:lang="en">identity</rdfs:label>
		<rdf:type
			rdf:resource="http://www.w3.org/2002/07/owl#FunctionalProperty" />
		<rdfs:domain rdf:resource="#Service" />
		<skos:definition xml:lang="en">
			The identity of the subject
		</skos:definition>
		<rdfs:comment xml:lang="en">This is the source that asserts the triples generated by the service</rdfs:comment>
	</owl:DatatypeProperty>
	
	<owl:DatatypeProperty rdf:ID="trustedSource">
		<rdfs:label xml:lang="en">trustedSource</rdfs:label>
		<rdfs:domain rdf:resource="#Service" />
		<skos:definition xml:lang="en">
			A source trusted by the subject
		</skos:definition>
		<rdfs:comment xml:lang="en">Typically a service takes its configuration from the trusted sources</rdfs:comment>
	</owl:DatatypeProperty>

</rdf:RDF>